more comments + shorter proof for Language.mem_kstar using Language.mem_pow

FormaleSystemeInLean/LectureAndExercise/List.lean
@@ -17,11 +17,16 @@ theorem List.removeAll_nil_flatten [BEq α] : ∀ (l : List (List α)), (l.remov
       have a_eq : ¬(a = []) := by simp_all
       rw [List.flatten_cons, ih]
       rfl
-
+/--
+Eliminates duplicates from a list, keeping the rightmost occurrence. (Implementation copied from...)
+-/
 def List.removeDups [DecidableEq α] : List α -> List α
   | [] => []
   | hd::tl => if hd ∈ tl then tl.removeDups else hd::(tl.removeDups)
 
+/--
+Removing duplicates from a list does not change the elements contained in it.
+-/
 theorem List.mem_removeDups [DecidableEq α] (l : List α) : ∀ a, a ∈ l ↔ a ∈ l.removeDups := by
   induction l with
   | nil =>
@@ -39,3 +44,58 @@ theorem List.mem_removeDups [DecidableEq α] (l : List α) : ∀ a, a ∈ l ↔ 
         simpa using aux
       . simp only [a_eq, false_or]
     . simp only [b_mem, ite_false, List.mem_cons, ih]
+
+instance List.decidableInfix [DecidableEq α] : ∀ (k l : List α), Decidable (k <:+: l)
+  | [], l => by
+    apply isTrue
+    unfold List.IsInfix
+    exists l, []
+    simp only [append_nil]
+  | a :: k, [] => by
+    apply isFalse
+    unfold List.IsInfix
+    simp only [append_assoc, cons_append, append_eq_nil_iff, reduceCtorEq, and_false, exists_const,
+      not_false_eq_true]
+  | k, b :: l =>
+    letI := k.decidableInfix l
+    @decidable_of_decidable_of_iff (k <+: b :: l ∨ k <:+: l) _ _
+      infix_cons_iff.symm
+
+def List.isInfixOf [DecidableEq α] : List α → List α → Bool
+  | [], _ => true
+  | _, [] => false
+  | a::s, b::k => a::s <+: b::k ∨ s.isInfixOf k
+
+theorem List.isInfixOf_cons [DecidableEq α] (k l : List α) (a : α) : k.isInfixOf l → k.isInfixOf (a::l) := by
+  intro h
+
+  sorry
+
+theorem List.isInfixOf_iff_Infix [DecidableEq α] (k l : List α) : k.isInfixOf l ↔ k <:+: l := by
+  induction l generalizing k with
+  | nil =>
+    cases  k_eq : k with
+    | nil =>
+      simp only [infix_rfl, iff_true]
+      rfl
+    | cons hd tl =>
+      simp only [infix_nil, reduceCtorEq, iff_false, Bool.not_eq_true]
+      rfl
+  | cons b s ih =>
+    constructor
+    . intro h
+      unfold isInfixOf at h
+
+      sorry
+    . intro h
+      unfold isInfixOf
+      cases k_eq : k with
+      | nil =>
+        simp only
+      | cons hd tl =>
+        simp
+        rcases h with ⟨f, g, x⟩
+        by_cases hb : hd = b
+        . sorry
+        .
+          sorry
